src/high/abstract_state.v
@@ -7,5 +7,7 @@ Class AbstractState ST `{Countable ST} := {
   abs_state_preorder :> PreOrder abs_state_relation;
 }.
 
+Global Hint Mode AbstractState ! - - : typeclass_instances.
+
 Instance abstract_state_sqsubseteq `{AbstractState ST} : SqSubsetEq ST :=
   abs_state_relation.
